src/Lib/DWT/VST/Der_write_TL.v
@@ -10,13 +10,7 @@ Require Import
         Exec.Ber_tlv_length_serialize Exec.Ber_tlv_tag_serialize Types.
 
 Definition composites :=
-  composites ++ (match find_cs dummy._dummy dummy.composites with
-                 | Some r => [r]
-                 | None => []
-                 end) ++ (match find_cs dummy._application_specific_key dummy.composites with
-                 | Some r => [r]
-                 | None => []
-                 end) .
+  composites ++ [Composite dummy._application_specific_key Struct nil noattr].
 
 Definition Vprog : varspecs. 
 Proof.
